Source/Dafny/Compilers/Compiler-js.cs
@@ -333,7 +333,7 @@ namespace Microsoft.Dafny.Compilers {
         w0.WriteLine("return this._d");
       }
 
-      // query properties
+      // create methods
       var i = 0;
       foreach (var ctor in dt.Ctors) {
         if (ctor.IsGhost) {
@@ -382,6 +382,9 @@ namespace Microsoft.Dafny.Compilers {
       // query properties
       i = 0;
       foreach (var ctor in dt.Ctors) {
+        if (ctor.IsGhost) {
+          continue;
+        }
         // get is_Ctor0() { return _D is Dt_Ctor0; }
         wr.WriteLine("get is_{0}() {{ return this.$tag === {1}; }}", ctor.CompileName, i);
         i++;
@@ -397,15 +400,20 @@ namespace Microsoft.Dafny.Compilers {
           var w = wr.NewNamedBlock("static *AllSingletonConstructors_()");
           foreach (var ctor in dt.Ctors) {
             Contract.Assert(ctor.Formals.Count == 0);
-            w.WriteLine("yield {0}.create_{1}({2});", DtT_protected, ctor.CompileName, dt is CoDatatypeDecl ? "null" : "");
+            if (ctor.IsGhost) {
+              w.WriteLine("yield {0};", ForcePlaceboValue(UserDefinedType.FromTopLevelDecl(dt.tok, dt), w, dt.tok));
+            } else {
+              w.WriteLine("yield {0}.create_{1}({2});", DtT_protected, ctor.CompileName, dt is CoDatatypeDecl ? "null" : "");
+            }
           }
         }
       }
 
       // destructors
       foreach (var ctor in dt.Ctors) {
-        foreach (var dtor in ctor.Destructors) {
-          if (dtor.EnclosingCtors[0] == ctor) {
+        foreach (var dtor in ctor.Destructors.Where(dtor => dtor.EnclosingCtors[0] == ctor)) {
+          var compiledConstructorCount = dtor.EnclosingCtors.Count(constructor => !constructor.IsGhost);
+          if (compiledConstructorCount != 0) {
             var arg = dtor.CorrespondingFormals[0];
             if (!arg.IsGhost && arg.HasName) {
               // datatype:   get dtor_Dtor0() { return this.Dtor0; }
@@ -502,9 +510,13 @@ namespace Microsoft.Dafny.Compilers {
         var wDefault = wr.NewBlock(")");
         wDefault.Write("return ");
         var groundingCtor = dt.GetGroundingCtor();
-        var nonGhostFormals = groundingCtor.Formals.Where(f => !f.IsGhost).ToList();
-        var arguments = Util.Comma(nonGhostFormals, f => DefaultValue(f.Type, wDefault, f.tok));
-        EmitDatatypeValue(dt, groundingCtor, dt is CoDatatypeDecl, arguments, wDefault);
+        if (groundingCtor.IsGhost) {
+          wDefault.Write(ForcePlaceboValue(UserDefinedType.FromTopLevelDecl(dt.tok, dt), wDefault, dt.tok));
+        } else {
+          var nonGhostFormals = groundingCtor.Formals.Where(f => !f.IsGhost).ToList();
+          var arguments = Util.Comma(nonGhostFormals, f => DefaultValue(f.Type, wDefault, f.tok));
+          EmitDatatypeValue(dt, groundingCtor, dt is CoDatatypeDecl, arguments, wDefault);
+        }
         wDefault.WriteLine(";");
       }
 
